ActRulesProofsScript.sml
@@ -7,7 +7,7 @@ open preamble
      AuxRulesEquivProofsTheory
      ActRulesSpecTheory
      ActRulesBoolTheory
-                      
+                          
 
 val _ = new_theory "ActRulesProofs";
      
@@ -88,37 +88,56 @@ val Logical_transfer_to_Functional_Transfer = Q.store_thm("Logical_transfer_to_F
              Logical_subpile1_IMP_TheFunctional,Logical_subpile2_IMP_TheFunctional,TRANSFER_Auxiliary_def,
 	     GET_CAND_PILE_MEM,Valid_PileTally_def,MEM_MAP]);   
         
-     
+       
 val Functional_to_Logical_elect = Q.store_thm("Functional_to_Logical_elect",
  `! st qu l j1 j2. ELECT_dec (qu,st,l) j1 j2 ==> ELECT (qu,st,l) j1 j2`,
   
- Cases_on `j1`
-  >- (Cases_on `j2`   
-     >- (REPEAT STRIP_TAC >> PairCases_on`p` >> PairCases_on`p'`
-      >> fs[ELECT_dec_def,ELECT_def] 
-       >> MAP_EVERY qexists_tac [`DROP (LENGTH p3) p'3`]
+ Cases_on `j1`  
+  >- (Cases_on `j2`     
+     >- (REPEAT STRIP_TAC >> PairCases_on`p` >> PairCases_on`p'`  
+      >> fs[ELECT_dec_def,ELECT_def]   
+       >> MAP_EVERY qexists_tac [`DROP (LENGTH p3) p'3`] 
         >> `p'3 = p3 ++ (DROP (LENGTH p3) p'3)` by
           metis_tac[ELECT_Auxiliary_dec_def,TAKE_DROP,DROP_LENGTH,TAKE_DROP_LENGTH_BACKLOG,APPEND_11] 
-       >> metis_tac[Functional_ElectAux_to_Logical,functional_to_logical_update_pile_ACT,
-                    ELECT_Auxiliary_dec_def,NULL,NULL_EQ])    
+        >> `!c. MEM c (DROP (LENGTH p3) p'3) ==> MEM c (MAP FST p2)`
+           by metis_tac[ELECT_Auxiliary_dec_def,MEM,MEM_APPEND,Valid_PileTally_def,PileTally_DEC1_to_PileTally,
+              PileTally_DEC2_IMP_PileTally,Valid_Init_CandList_def,eqe_list_dec2_verified,
+             list_eqe_dec_MEM1,Valid_PileTally_def,Valid_PileTally_def,
+             Logical_list_MEM_VICE_VERCA_TheFunctional,eqe_list_dec2_verified]
+        >> `!c. MEM c (DROP (LENGTH p3) p'3) ==> MEM c (MAP FST p'2)`
+           by metis_tac[ELECT_Auxiliary_dec_def,MEM,MEM_APPEND,Valid_PileTally_def,PileTally_DEC1_to_PileTally,
+              PileTally_DEC2_IMP_PileTally,Valid_Init_CandList_def,eqe_list_dec2_verified,
+             list_eqe_dec_MEM1,Valid_PileTally_def,Valid_PileTally_def,
+             Logical_list_MEM_VICE_VERCA_TheFunctional,eqe_list_dec2_verified]
+        >> metis_tac[Functional_ElectAux_to_Logical,ELECT_Auxiliary_dec_def,ALL_NON_EMPTY_def,ALL_NON_ZERO_def,
+         Functional_AllNonEmpty_to_Logical,Functional_AllNonZero_to_Logical,
+         GET_CAND_PILE_MEM,Functional_AllNonEmpty_to_Logical,GET_CAND_PILE_MEM,
+         EVERY_CAND_HAS_ONE_PILE,PileTally_to_PileTally_DEC1,PileTally_to_PileTally_DEC2,
+         Valid_PileTally_def,Valid_PileTally_def,Logical_list_MEM_VICE_VERCA_TheFunctional,
+         eqe_list_dec2_verified,EVERY_CAND_HAS_ONE_PILE,PileTally_to_PileTally_DEC1,
+         PileTally_to_PileTally_DEC2,Valid_PileTally_def,Valid_PileTally_def,
+         Logical_list_MEM_VICE_VERCA_TheFunctional,eqe_list_dec2_verified,functional_to_logical_update_pile_ACT])
      >- rfs[ELECT_dec_def]) 
   >- rfs[ELECT_dec_def]);     
-  
-  
+    
+      
 val Logical_to_Functional_elect = Q.store_thm ("Logical_to_Functional_elect",
  `! st qu l j1 j2. ELECT (qu,st,l) j1 j2 ==> ELECT_dec (qu,st,l) j1 j2`,
 
  REPEAT STRIP_TAC  
-  >> fs[ELECT_def,ELECT_dec_def]  
-  >> fs[Logical_ElectAux_to_Functional]  
-  >> fs[Logical_ElectAux_to_Functional]  
-  >> `DROP (LENGTH bl) (bl ++ l1) = l1` by metis_tac[DROP_LENGTH]  
-  >> rw[]  
-  >> rfs[ELECT_Auxiliary_def] 
-  >> `!c. MEM c l1 ==> MEM c (MAP FST np)` by metis_tac [ELECT_Auxiliary_def,MEM,Valid_PileTally_def]
-  >> metis_tac[logical_to_functional_update_pile_ACT]) 
- 
- 
+  >> fs[ELECT_def,ELECT_dec_def] 
+  >> `DROP (LENGTH bl) (bl ++ l1) = l1` by metis_tac[DROP_LENGTH]
+  >> fs[Logical_ElectAux_to_Functional] 
+  >> rfs[ELECT_Auxiliary_def]  
+  >> `!c. MEM c l1 ==> MEM c (MAP FST p)`
+       by metis_tac [ELECT_Auxiliary_def,MEM,Valid_PileTally_def]
+  >> `!c. MEM c l1 ==> MEM c (MAP FST np)`
+       by metis_tac [ELECT_Auxiliary_def,MEM,Valid_PileTally_def]
+  >> fs[logical_to_functional_update_pile_ACT]
+  >> metis_tac[Logical_AllNonZero_to_Functional,
+                MEM,ELECT_Auxiliary_def,Logical_AllNonEpty_to_Functional])   
+             
+  
 val Functional_Count_to_Logical = Q.store_thm("Functional_Count_to_Logical",
  `! st qu l j1 j2. COUNT_dec (qu,st,l) j1 j2 ==> COUNT (qu,st,l) j1 j2`,
  
@@ -141,32 +160,43 @@ val Logical_Count_to_Functional = Q.store_thm("Logical_Count_to_Functional",
                 Logical_CountAux_to_Functional,COUNT_Auxiliary_def]);
 
  
+val TRANSFER_EXCLUDED_Auxiliary_thm = Q.store_thm("TRANSFER_EXCLUDED_Auxiliary_thm",
+ `TRANSFER_EXCLUDED_Auxiliary_dec = TRANSFER_EXCLUDED_Auxiliary`,
+   simp[FUN_EQ_THM,Logical_TransferExcludedAux_to_Functional,Functional_TransferExcluded_Aux_to_Logical,
+        FORALL_PROD,EQ_IMP_THM]);
 
-val Logical_TransferExcluded_to_Functional = Q.store_thm("Logical_TransferExcluded_to_Functional",
- `!qu st l j1 j2. TRANSFER_EXCLUDED (qu,st,l) j1 j2 ==> TRANSFER_EXCLUDED_dec (qu,st,l) j1 j2`,
- 
-   fs[TRANSFER_EXCLUDED_dec_def,TRANSFER_EXCLUDED_def]);
-  
- 
-val Functional_TransferExcluded_to_Logical = Q.store_thm("Functional_TransferExcluded_to_Logical",
- `!qu st l j1 j2. TRANSFER_EXCLUDED_dec (qu,st,l) j1 j2 ==> TRANSFER_EXCLUDED_dec (qu,st,l) j1 j2`,
 
-    rw[]);
-   
-       
 val TRANSFER_EXCLUDED_thm = Q.store_thm("TRANSFER_EXCLUDED_thm",
    `TRANSFER_EXCLUDED_dec = TRANSFER_EXCLUDED`,
-  
-        (simp[FUN_EQ_THM]    
-         >> qx_gen_tac`params`   
-          >> PairCases_on`params`   
-           >>  Cases)  
-             >-( Cases   
-               >- (PairCases_on`p`   
+
+        (simp[FUN_EQ_THM]
+          >> qx_gen_tac`params`
+          >> PairCases_on`params`
+           >>  Cases)
+             >-(Cases
+               >- (PairCases_on`p`
                    >> PairCases_on `p'`
-		    >> simp[TRANSFER_EXCLUDED_dec_def,TRANSFER_EXCLUDED_def])  
-               >- simp[TRANSFER_EXCLUDED_dec_def,TRANSFER_EXCLUDED_def])           
-             >- simp[TRANSFER_EXCLUDED_dec_def,TRANSFER_EXCLUDED_def]);         
+                    >> simp[TRANSFER_EXCLUDED_dec_def,TRANSFER_EXCLUDED_def,TRANSFER_EXCLUDED_Auxiliary_thm])
+                     >- simp[TRANSFER_EXCLUDED_dec_def,TRANSFER_EXCLUDED_def,TRANSFER_EXCLUDED_Auxiliary_thm])
+                     >- simp[TRANSFER_EXCLUDED_dec_def,TRANSFER_EXCLUDED_def,TRANSFER_EXCLUDED_Auxiliary_thm]);
+
+
+ (*
+val TRANSFER_EXCLUDED_thm = Q.store_thm("TRANSFER_EXCLUDED_thm",
+   `TRANSFER_EXCLUDED_dec = TRANSFER_EXCLUDED`,
+
+        (simp[FUN_EQ_THM]
+          >> qx_gen_tac`params`
+          >> PairCases_on`params`
+           >>  Cases)
+             >-(Cases
+               >- (PairCases_on`p`
+                   >> PairCases_on `p'`
+                    >> simp[TRANSFER_EXCLUDED_dec_def,TRANSFER_EXCLUDED_def,TRANSFER_EXCLUDED_Auxiliary_thm])
+                     >- simp[TRANSFER_EXCLUDED_dec_def,TRANSFER_EXCLUDED_def,TRANSFER_EXCLUDED_Auxiliary_thm])
+                     >- simp[TRANSFER_EXCLUDED_dec_def,TRANSFER_EXCLUDED_def,TRANSFER_EXCLUDED_Auxiliary_thm]);
+
+*)
 
 
 val _ = export_theory ();
